src/canonize/pterm.lean
@@ -1,0 +1,232 @@
+import .nterm
+
+namespace polya
+
+open nterm
+
+variables {α : Type} [discrete_field α]
+variables {γ : Type} [coeff γ]
+variables [morph γ α] {ρ : dict α}
+
+structure xterm : Type :=
+(term : @nterm γ _)
+(exp : znum)
+
+namespace xterm
+
+def le (x y : @xterm γ _) : Prop := x.term ≤ y.term
+
+instance : has_le (@xterm γ _) := ⟨le⟩
+instance : decidable_rel (@xterm.le γ _) := by delta xterm.le; apply_instance
+
+def pow (x : @xterm γ _) (n : znum) : @xterm γ _ :=
+⟨x.term, x.exp * n⟩
+
+def of_nterm (x : @nterm γ _) : @xterm γ _ :=
+⟨x, 1⟩
+
+def to_nterm (x : @xterm γ _) : @nterm γ _ :=
+if x.exp = 0 then 1
+else if x.exp = 1 then x.term
+else x.term ^ x.exp
+
+def eval (ρ : dict α) (x : @xterm γ _) : α :=
+x.term.eval ρ ^ (x.exp : ℤ)
+
+theorem eval_def {x : @nterm γ _} {n : znum} :
+  eval ρ ⟨x, n⟩ = x.eval ρ ^ (n : ℤ) :=
+rfl
+
+theorem eval_to_nterm (x : @xterm γ _) :
+  x.to_nterm.eval ρ = x.eval ρ :=
+begin
+  unfold to_nterm, unfold eval,
+  by_cases h1 : x.exp = 0,
+  { simp [h1] },
+  { by_cases h2 : x.exp = 1,
+    { simp [h2] },
+    { simp [h1, h2] }}
+end
+
+theorem eval_to_nterm' :
+  @nterm.eval _ _ γ _ _ ρ ∘ xterm.to_nterm = xterm.eval ρ :=
+begin
+  unfold function.comp,
+  simp [eval_to_nterm]
+end
+
+theorem eval_pow {x : @xterm γ _} {n : znum} :
+  (x.pow n).eval ρ = x.eval ρ ^ (n : ℤ) :=
+by simp [pow, eval, fpow_mul] 
+
+end xterm
+
+structure pterm : Type :=
+(terms : list (@xterm γ _))
+
+namespace pterm
+
+def append (S1 S2 : @pterm γ _) : @pterm γ _ :=
+⟨S1.terms ++ S2.terms⟩
+
+instance : has_append (@pterm γ _) := ⟨append⟩
+
+theorem append_terms (S1 S2 : @pterm γ _) :
+  (S1 ++ S2).terms = S1.terms ++ S2.terms := rfl
+
+def pow (S : @pterm γ _) (n : znum) : @pterm γ _ :=
+if n = 0 then ⟨[]⟩
+else if n = 1 then S
+else ⟨S.terms.map (λ x, x.pow n)⟩
+
+def eval (ρ : dict α) (S : @pterm γ _) : α :=
+list.prod (S.terms.map (xterm.eval ρ))
+
+theorem eval_pow (S : @pterm γ _) (n : znum) :
+(S.pow n).eval ρ = S.eval ρ ^ (n : ℤ) :=
+begin
+  by_cases h : n = 0 ∨ n = 1,
+  { cases h with h h,
+    { simp [h, pow, eval] },
+    { simp [h, pow, eval] }},
+  { have h0 : ¬ n = 0, by { intro h0, apply h, left, exact h0 },
+    have h1 : ¬ n = 1, by { intro h1, apply h, right, exact h1 },
+    cases S with terms,
+    simp [h0, h1, pow, eval], 
+    induction terms with x xs ih,
+    { simp },
+    { simp [ih, mul_fpow, xterm.eval_pow] }
+  }
+end
+
+theorem eval_mul (S1 S2 : @pterm γ _) :
+  (S1 ++ S2).eval ρ = S1.eval ρ * S2.eval ρ :=
+begin
+  unfold eval,
+  simp only [append_terms],
+  rw [list.map_append],
+  apply list.prod_append 
+end
+
+def to_nterm (S : @pterm γ _) : @nterm γ _ :=
+prod (S.terms.map (xterm.to_nterm))
+
+theorem eval_to_nterm {S : @pterm γ _} :
+  S.eval ρ = S.to_nterm.eval ρ :=
+begin
+  cases S with terms,
+  unfold to_nterm, unfold eval,
+  rw [eval_prod, list.map_map],
+  rw xterm.eval_to_nterm'
+end
+
+def reduce_aux : @xterm γ _ → list (@xterm γ _) → list (@xterm γ _)
+| x []      := [x] --TODO
+| x (y::ys) :=
+  if x.term = y.term then
+    reduce_aux ⟨x.term, x.exp + y.exp⟩ ys
+  else if x.exp = 0 then
+    reduce_aux y ys
+  else
+    x::(reduce_aux y ys)
+  
+theorem eval_reduce_aux (x : @xterm γ _) (xs : list (@xterm γ _)) :
+  pterm.eval ρ ⟨reduce_aux x xs⟩ = pterm.eval ρ ⟨x::xs⟩ :=
+begin
+  revert x,
+  induction xs with y ys ih,
+  { simp [eval, reduce_aux] },
+  { intro x,
+    unfold eval,
+    rw [list.map_cons, list.prod_cons],
+    unfold eval at ih,
+    by_cases h1 : x.term = y.term,
+    { rw [list.map_cons, list.prod_cons],
+      rw [← mul_assoc],
+      unfold xterm.eval,
+      rw [h1, ← fpow_add],
+      { norm_cast,
+        rw [← xterm.eval_def, ← list.prod_cons, ← list.map_cons],
+        rw [← ih],
+        simp [reduce_aux, h1] },
+      { sorry }}, -- TODO: introduce hypothesis
+    by_cases h2 : x.exp = 0,
+    { rw [list.map_cons, list.prod_cons],
+      unfold xterm.eval,
+      rw_mod_cast [h2, fpow_zero],
+      rw [← xterm.eval_def, ← list.prod_cons, ← list.map_cons],
+      simp [reduce_aux, h1, h2, ih], refl
+    },
+    conv {
+      to_lhs,
+      simp [reduce_aux, h1, h2]
+    },
+    simp [ih]
+  }
+end
+
+def reduce (S : @pterm γ _) : @pterm γ _ :=
+match S.terms with
+| []      := ⟨[]⟩
+| (x::xs) := ⟨reduce_aux x xs⟩
+end
+ 
+theorem eval_reduce {S : @pterm γ _} :
+  S.eval ρ = S.reduce.eval ρ :=
+begin
+  cases S with terms,
+  cases terms with x xs,
+  { simp [reduce] },
+  { simp [reduce, eval_reduce_aux] }
+end
+
+def sort (S : @pterm γ _) : @pterm γ _ :=
+⟨S.terms.merge_sort (≤)⟩
+
+theorem eval_sort {S : @pterm γ _} :
+  S.eval ρ = S.sort.eval ρ :=
+begin
+  unfold eval, unfold sort,
+  apply list.prod_eq_of_perm,
+  apply list.perm_map,
+  apply list.perm.symm,
+  apply list.perm_merge_sort
+end
+
+end pterm
+
+namespace nterm
+
+def to_pterm : @nterm γ _ → @pterm γ _
+| (mul x y) := x.to_pterm ++ y.to_pterm
+| (pow x n) := x.to_pterm.pow n
+| x := ⟨[⟨x, 1⟩]⟩
+
+theorem eval_to_pterm {x : @nterm γ _} :
+  nterm.eval ρ x = pterm.eval ρ x.to_pterm :=
+begin
+  induction x with i c x y ihx ihy x y ihx ihy x n ihx,
+  { simp [to_pterm, nterm.eval, pterm.eval, xterm.eval] },
+  { simp [to_pterm, nterm.eval, pterm.eval, xterm.eval] },
+  { simp [to_pterm, nterm.eval, pterm.eval, xterm.eval] },
+  { unfold to_pterm, unfold eval,
+    rw [pterm.eval_mul, ihx, ihy] },
+  { unfold to_pterm, unfold eval,
+    rw [pterm.eval_pow, ihx] }
+
+end
+
+def norm (x : @nterm γ _) : @nterm γ _ :=
+x.to_pterm.sort.reduce.to_nterm
+
+theorem correctness {x : @nterm γ _} :
+  x.eval ρ = x.norm.eval ρ :=
+calc
+  x.eval ρ = pterm.eval ρ x.to_pterm             : eval_to_pterm
+       ... = pterm.eval ρ x.to_pterm.sort        : pterm.eval_sort
+       ... = pterm.eval ρ x.to_pterm.sort.reduce : pterm.eval_reduce
+       ... = nterm.eval ρ x.norm                 : pterm.eval_to_nterm
+
+end nterm
+
+end polya
