src/canonize/test.lean
@@ -18,7 +18,14 @@ set_option profiler true
 /- debug -/
 set_option trace.app_builder true
 
+--sterm tests
 run_cmd test `( x - x )
 run_cmd test `( x * (1 / 10 : ℚ) + x * (1 / 10 : ℚ) - x * (1 / 5 : ℚ))
 run_cmd test `( x * (3 : ℚ) + y * (1 : ℚ) - x * y * (2 : ℚ) - y * (2 : ℚ) )
 run_cmd test `( x * y * (3 : ℚ) - x * y * (4 : ℚ) )
+
+--pterm tests
+run_cmd test `( x * x)
+run_cmd test `( x / x )
+run_cmd test `( (x * y) ^ 3 / x ^ 2 )
+
